theories/protocol_agreement.v
@@ -19,49 +19,41 @@ From hazel               Require Import lib lang ieff.
 Section protocol_agreement.
 Context `{!irisG eff_lang Σ}.
 
-(* Comment: In defining [protocol_agreement], we could have followed a
-            different approach by removing the fancy update modalities
-            and letting the user decide when to introduce them.
-            Here we choose to follow the same approach as in the
-            definition of [ewp]. *)
+Definition protocol_agreement v Ψ (Φ : val -d> iPropO Σ) :=
+  let: P := iEff_car Ψ in
+  (∃ Q, P v Q ∗ (∀ w, Q w -∗ Φ w))%I.
+Arguments protocol_agreement _%V _%ieff _%I.
 
-Definition protocol_agreement E v Ψ (Φ : val -d> iPropO Σ) :=
-  (|={E,∅}=>
-    let: P := iEff_car Ψ in
-    ∃ Q, P v Q ∗ (∀ w, Q w ={∅,E}=∗ Φ w))%I.
-Arguments protocol_agreement _ _%V _%ieff _%I.
-
-Global Instance protocol_agreement_ne E v n :
-  Proper ((dist n) ==> (dist n) ==> (dist n)) (protocol_agreement E v).
+Global Instance protocol_agreement_ne v n :
+  Proper ((dist n) ==> (dist n) ==> (dist n)) (protocol_agreement v).
 Proof.
   intros ??? ???. rewrite /protocol_agreement.
   by repeat (apply H || apply H0 || f_equiv).
 Qed.
-Global Instance protocol_agreement_proper E v :
-  Proper ((≡) ==> (≡) ==> (≡)) (protocol_agreement E v).
+Global Instance protocol_agreement_proper v :
+  Proper ((≡) ==> (≡) ==> (≡)) (protocol_agreement v).
 Proof.
   intros ??? ???. apply equiv_dist=>n.
   apply protocol_agreement_ne; by apply equiv_dist.
 Qed.
 
-Lemma protocol_agreement_bottom E v Φ :
-  protocol_agreement E v ⊥ Φ ≡ (|={E,∅}=> False)%I.
+Lemma protocol_agreement_bottom v Φ :
+  protocol_agreement v ⊥ Φ ≡ False%I.
 Proof.
-  rewrite /protocol_agreement. f_equiv.
+  rewrite /protocol_agreement.
   iSplit; iIntros "H"; [|done]. by iDestruct "H" as (Q) "[H _]".
 Qed.
 
-Lemma protocol_agreement_tele {TT1 TT2 : tele} E v
+Lemma protocol_agreement_tele {TT1 TT2 : tele} v
   (v' : TT1 →       val) (P : TT1 →       iProp Σ)
   (w' : TT1 → TT2 → val) (Q : TT1 → TT2 → iProp Σ) Φ :
-  protocol_agreement E v
+  protocol_agreement v
     (>>.. x >> ! (v' x)   {{ P x   }};
      <<.. y << ? (w' x y) {{ Q x y }}) Φ ≡
-  (|={E,∅}=>
-    (∃.. x, ⌜ v = v' x ⌝ ∗ P x ∗
-      (∀.. y, Q x y ={∅,E}=∗ Φ (w' x y))))%I.
+  (∃.. x, ⌜ v = v' x ⌝ ∗ P x ∗
+    (∀.. y, Q x y -∗ Φ (w' x y)))%I.
 Proof.
-  rewrite /protocol_agreement. f_equiv. iSplit.
+  rewrite /protocol_agreement. iSplit.
 
   - iIntros "H". iDestruct "H" as (Q') "[HP HQ']".
     rewrite iEffPre_texist_eq iEffPre_base_eq /iEffPre_base_def.
@@ -79,144 +71,220 @@ Proof.
       iDestruct "HQ'" as (y) "[<- HQ']". by iApply "HQ".
 Qed.
 
-Lemma protocol_agreement_tele' (TT1 TT2 : tele) E v
+Lemma protocol_agreement_tele' (TT1 TT2 : tele) v
   (v' : TT1 -t>         val) (P : TT1 -t>         iProp Σ)
   (w' : TT1 -t> TT2 -t> val) (Q : TT1 -t> TT2 -t> iProp Σ) Φ :
-  protocol_agreement E v
+  protocol_agreement v
     (>>.. x >> !           (tele_app v' x)
                {{          (tele_app P  x)   }};
      <<.. y << ? (tele_app (tele_app w' x) y)
                {{ tele_app (tele_app Q  x) y }}) Φ ≡
-  (|={E,∅}=>
-     ∃.. x, ⌜ v = tele_app v' x ⌝ ∗ tele_app P x ∗
-       ∀.. y, tele_app (tele_app Q  x) y ={∅,E}=∗
-           Φ (tele_app (tele_app w' x) y))%I.
-Proof. by rewrite (protocol_agreement_tele E _ (tele_app v') (tele_app P)
+  (∃.. x, ⌜ v = tele_app v' x ⌝ ∗ tele_app P x ∗
+     ∀.. y, tele_app (tele_app Q  x) y -∗
+         Φ (tele_app (tele_app w' x) y))%I.
+Proof. by rewrite (protocol_agreement_tele _ (tele_app v') (tele_app P)
                   (λ x y, tele_app (tele_app w' x) y)
                   (λ x y, tele_app (tele_app Q  x) y)).
 Qed.
 
-Lemma protocol_agreement_marker_tele {TT1 TT2 : tele} E f v
+Lemma protocol_agreement_marker_tele {TT1 TT2 : tele} f v
   (v' : TT1 →       val) (P : TT1 →       iProp Σ)
   (w' : TT1 → TT2 → val) (Q : TT1 → TT2 → iProp Σ) Φ :
-  protocol_agreement E v
+  protocol_agreement v
     (f #> (>>.. x >> !    (v' x  )  {{ P x   }};
            <<.. y << ?    (w' x y)  {{ Q x y }})) Φ ≡
-  protocol_agreement E v
+  protocol_agreement v
           (>>.. x >> ! (f (v' x  )) {{ P x   }};
            <<.. y << ? (  (w' x y)) {{ Q x y }})  Φ.
 Proof. by rewrite iEff_marker_tele. Qed.
 
-Lemma protocol_agreement_marker_intro E f v Ψ Φ :
-  protocol_agreement E v Ψ Φ ⊢ protocol_agreement E (f v) (f #> Ψ) Φ.
+Lemma protocol_agreement_marker_intro f v Ψ Φ :
+  protocol_agreement v Ψ Φ ⊢ protocol_agreement (f v) (f #> Ψ) Φ.
 Proof.
   rewrite /protocol_agreement iEff_marker_eq.
-  iIntros "H". iMod "H" as (Q) "[He HQ]".
+  iIntros "H". iDestruct "H" as (Q) "[He HQ]".
   iExists Q. iFrame. iExists v. by iFrame.
 Qed.
 
-Lemma protocol_agreement_marker_elim E f {Hf: Inj (=) (=) f} v Ψ Φ :
-  protocol_agreement E (f v) (f #> Ψ) Φ ⊢ protocol_agreement E v Ψ Φ.
+Lemma protocol_agreement_marker_elim f {Hf: Inj (=) (=) f} v Ψ Φ :
+  protocol_agreement (f v) (f #> Ψ) Φ ⊢ protocol_agreement v Ψ Φ.
 Proof.
   iIntros "H". rewrite iEff_marker_eq /protocol_agreement //=.
-  iMod "H" as (Q) "[HP HQ]".
+  iDestruct "H" as (Q) "[HP HQ]".
   iDestruct "HP" as (w') "[% HP]". rewrite (Hf _ _ H).
-  iModIntro. iExists Q. by iFrame.
+  iExists Q. by iFrame.
 Qed.
 
-Lemma protocol_agreement_sum_assoc E v Ψ1 Ψ2 Ψ3 Φ :
-  protocol_agreement E v (Ψ1 <+> (Ψ2 <+> Ψ3)) Φ ≡
-    protocol_agreement E v ((Ψ1 <+> Ψ2) <+> Ψ3) Φ.
+Lemma protocol_agreement_marker_elim' f v Ψ Φ :
+  protocol_agreement v (f #> Ψ) Φ ⊢ ∃ w, ⌜ v = f w ⌝ ∗ protocol_agreement w Ψ Φ.
+Proof.
+  iIntros "H". rewrite iEff_marker_eq /protocol_agreement //=.
+  iDestruct "H" as (Q) "[HP HQ]". iDestruct "HP" as (w) "[-> HP]".
+  iExists w. iSplit; [done|]. iExists Q. by iFrame.
+Qed.
+
+Lemma protocol_agreement_sum_assoc v Ψ1 Ψ2 Ψ3 Φ :
+  protocol_agreement v (Ψ1 <+> (Ψ2 <+> Ψ3)) Φ ≡
+    protocol_agreement v ((Ψ1 <+> Ψ2) <+> Ψ3) Φ.
 Proof. by rewrite iEff_sum_assoc. Qed.
 
-Lemma protocol_agreement_sum_comm E v Ψ1 Ψ2 Φ :
-  protocol_agreement E v (Ψ2 <+> Ψ1) Φ ≡ protocol_agreement E v (Ψ1 <+> Ψ2) Φ.
+Lemma protocol_agreement_sum_comm v Ψ1 Ψ2 Φ :
+  protocol_agreement v (Ψ2 <+> Ψ1) Φ ≡ protocol_agreement v (Ψ1 <+> Ψ2) Φ.
 Proof. by rewrite iEff_sum_comm. Qed.
 
-Lemma protocol_agreement_sum_intro_l E v Ψ1 Ψ2 Φ :
-  protocol_agreement E v Ψ1 Φ ⊢ protocol_agreement E v (Ψ1 <+> Ψ2) Φ.
+Lemma protocol_agreement_sum_intro_l v Ψ1 Ψ2 Φ :
+  protocol_agreement v Ψ1 Φ ⊢ protocol_agreement v (Ψ1 <+> Ψ2) Φ.
 Proof.
   rewrite /protocol_agreement iEff_sum_eq.
-  iIntros "H". iMod "H" as (Q) "[He HQ]". iExists Q. by iFrame.
+  iIntros "H". iDestruct "H" as (Q) "[He HQ]". iExists Q. by iFrame.
 Qed.
 
-Lemma protocol_agreement_sum_intro_r E v Ψ1 Ψ2 Φ :
-  protocol_agreement E v Ψ2 Φ ⊢ protocol_agreement E v (Ψ1 <+> Ψ2) Φ.
+Lemma protocol_agreement_sum_intro_r v Ψ1 Ψ2 Φ :
+  protocol_agreement v Ψ2 Φ ⊢ protocol_agreement v (Ψ1 <+> Ψ2) Φ.
 Proof.
   iIntros "H". rewrite protocol_agreement_sum_comm.
   by iApply protocol_agreement_sum_intro_l.
 Qed.
 
-Lemma protocol_agreement_sum_elim E (f g : val → val)
-  {Hf: Marker f} {Hg: Marker g} {Hfg: DisjRange f g} v Ψ1 Ψ2 Φ :
-  protocol_agreement E v ((f #> Ψ1) <+> (g #> Ψ2)) Φ ⊢
-    (protocol_agreement E v (f #> Ψ1) Φ) ∨
-    (protocol_agreement E v (g #> Ψ2) Φ).
+Lemma protocol_agreement_sum_elim v Ψ1 Ψ2 Φ :
+  protocol_agreement v (Ψ1 <+> Ψ2) Φ ⊢
+    (protocol_agreement v Ψ1 Φ) ∨ (protocol_agreement v Ψ2 Φ).
 Proof.
-  iAssert (∀ (f g : val → val) (Hfg: DisjRange f g) v Ψ1 Ψ2,
-    (protocol_agreement E (f v) ((f #> Ψ1) <+> (g #> Ψ2)) Φ -∗
-      (protocol_agreement E (f v) (f #> Ψ1) Φ)))%I
-  as "Haux".
-  { clear Hfg Hf Hg f g v Ψ1 Ψ2. iIntros (f g Hfg v Ψ1 Ψ2) "H".
-    rewrite iEff_marker_eq iEff_sum_eq /protocol_agreement //=.
-    iMod "H" as (Q) "[HP HQ]". iDestruct "HP" as "[HP|HP]".
-    - iModIntro. iDestruct "HP" as (v') "[% HP]".
-      iExists Q. iFrame. iExists v'. by iFrame.
-    - iClear "HQ". iDestruct "HP" as (v') "[% _]".
-      by destruct (disj_range v v' H). }
-
-  iIntros "H".
-  case (@marker_dec_range _ _ _ _ f Hf v) as [(v' & Hv')|Hf']; [|
-  case (@marker_dec_range _ _ _ _ g Hg v) as [(v' & Hv')|Hg']];
-  try inversion Hv'.
-  { iLeft. iSpecialize ("Haux" $! f g Hfg). by iApply "Haux". }
-  { iRight. rewrite protocol_agreement_sum_comm.
-    have Hgf: (DisjRange g f). by apply DisjRange_comm.
-    iSpecialize ("Haux" $! g f Hgf). by iApply "Haux". }
-  { iLeft. rewrite iEff_sum_eq iEff_marker_eq.
-    iMod "H" as (Q) "[HP _]". iDestruct "HP" as "[HP|HP]";
-    iDestruct "HP" as (w) "[-> _]"; [case (Hf' w)|case (Hg' w)]; done. }
+  iIntros "H". iDestruct "H" as (Q) "[HP HQ]".
+  rewrite iEff_sum_eq. iDestruct "HP" as "[HP|HP]".
+  { iLeft;  iExists Q; by iFrame. }
+  { iRight; iExists Q; by iFrame. }
 Qed.
 
-Lemma protocol_agreement_strong_mono E1 E2 v (Ψ1 Ψ2 : iEff Σ) Φ1 Φ2 :
-  E1 ⊆ E2 →
-  (protocol_agreement E1 v Ψ1 Φ1
-     -∗ Ψ1 ⊑ Ψ2 -∗ (∀ v, Φ1 v ={E2}=∗ Φ2 v) -∗
-   protocol_agreement E2 v Ψ2 Φ2)%ieff.
+Lemma protocol_agreement_mono v (Ψ : iEff Σ) Φ1 Φ2 :
+  (protocol_agreement v Ψ Φ1 -∗ (∀ w, Φ1 w -∗ Φ2 w) -∗
+   protocol_agreement v Ψ Φ2)%ieff.
 Proof.
-  iIntros (HE) "Hprot_agr #HΨ HΦ2".
-  iMod (fupd_intro_mask' E2 E1) as "Hclose"; first done.
-  iMod "Hprot_agr" as (Q) "[HP HΦ1]".
-  iExists Q. iSplitL "HP". { by iApply "HΨ". }
-  iModIntro. iIntros (w) "HQ". iSpecialize ("HΦ1" with "HQ").
-  iMod "HΦ1". iMod "Hclose". by iApply "HΦ2".
-Qed.
-
-Lemma protocol_agreement_mono E v (Ψ1 Ψ2 : iEff Σ) Φ :
-  (protocol_agreement E v Ψ1 Φ -∗ Ψ1 ⊑ Ψ2 -∗
-   protocol_agreement E v Ψ2 Φ)%ieff.
-Proof.
-  iIntros "H #HΨ".
-  by iApply (protocol_agreement_strong_mono with "H"); auto.
-Qed.
-
-Lemma protocol_agreement_mono' E v Ψ Φ1 Φ2 :
-  (protocol_agreement E v Ψ Φ1 -∗ (∀ w, Φ1 w ={E}=∗ Φ2 w) -∗
-   protocol_agreement E v Ψ Φ2)%ieff.
-Proof.
-  iIntros "H HΦ".
-  iApply (protocol_agreement_strong_mono with "H"); auto.
-  by iApply iEff_le_refl.
-Qed.
-
-Lemma protocol_agreement_mask_mono E1 E2 v Ψ Φ :
-  E1 ⊆ E2 →
-    protocol_agreement E1 v Ψ Φ -∗
-    protocol_agreement E2 v Ψ Φ.
-Proof.
-  iIntros (HE) "H".
-  iApply (protocol_agreement_strong_mono with "H"); auto.
-  { by iApply iEff_le_refl. }
+  iIntros "Hprot_agr HΦ2". iDestruct "Hprot_agr" as (Φ0) "[HP HΦ1]".
+  iExists Φ0. iFrame. iIntros (w) "HΦ0". iApply "HΦ2". by iApply "HΦ1".
 Qed.
 
 End protocol_agreement.
+
+
+(** * Protocol Ordering. *)
+
+Program Definition iEff_le {Σ} : iEffO -n> iEffO -n> iPropO Σ :=
+  λne Ψ1 Ψ2,
+    (□ (∀ v Φ, protocol_agreement v Ψ1 Φ -∗ protocol_agreement v Ψ2 Φ))%I.
+Next Obligation. intros ??????. repeat (apply iEff_car_ne || f_equiv); done. Defined.
+Next Obligation. intros ??????. simpl. repeat (apply iEff_car_ne || f_equiv); done. Defined.
+(*Arguments iEff_le {_} _%ieff _%ieff.*)
+Instance: Params (@iEff_le) 3 := {}.
+
+Infix "⊑" := (iEff_le) (at level 70, only parsing) : ieff_scope.
+
+Section protocol_ordering.
+Context {Σ : gFunctors}.
+
+Global Instance iEff_le_ne n :
+  Proper ((dist n) ==> (dist n)) (iEff_le (Σ:=Σ)).
+Proof.
+  rewrite /iEff_le. intros ????.
+  repeat (apply iEff_car_ne || f_equiv); done.
+Qed.
+Global Instance iEff_le_proper :  Proper ((≡) ==> (≡)) (iEff_le (Σ:=Σ)).
+Proof.
+  intros ????. apply equiv_dist=>n; apply iEff_le_ne; by apply equiv_dist.
+Qed.
+
+Lemma iEff_le_bottom (Ψ : iEff Σ) : ⊢ (⊥ ⊑ Ψ)%ieff.
+Proof. iModIntro. iIntros (v Φ) "H". by rewrite protocol_agreement_bottom. Qed.
+
+Lemma iEff_le_refl (Ψ : iEff Σ) : ⊢ (Ψ ⊑ Ψ)%ieff.
+Proof. iModIntro. by iIntros (v Φ) "H". Qed.
+
+Lemma iEff_le_trans (Ψ1 Ψ2 Ψ3 : iEff Σ) : (Ψ1 ⊑ Ψ2 -∗ Ψ2 ⊑ Ψ3 -∗ Ψ1 ⊑ Ψ3)%ieff.
+Proof.
+  iIntros "#H12 #H23". iModIntro. iIntros (v Φ) "H1".
+  iApply "H23". by iApply "H12".
+Qed.
+
+Lemma iEff_le_sum_l (Ψ1 Ψ2 : iEff Σ) : ⊢ (Ψ1 ⊑ Ψ1 <+> Ψ2)%ieff.
+Proof. iModIntro. iIntros (v Φ) "H". by iApply protocol_agreement_sum_intro_l. Qed.
+
+Lemma iEff_le_sum_r (Ψ1 Ψ2 : iEff Σ) : ⊢ (Ψ2 ⊑ Ψ1 <+> Ψ2)%ieff.
+Proof. rewrite (iEff_sum_comm Ψ1 Ψ2). by iApply iEff_le_sum_l. Qed.
+
+Lemma iEff_le_sum (Ψ1 Ψ2 Ψ1' Ψ2' : iEff Σ) :
+  (Ψ1 ⊑ Ψ1' -∗ Ψ2 ⊑ Ψ2' -∗ Ψ1 <+> Ψ2 ⊑ Ψ1' <+> Ψ2')%ieff.
+Proof.
+  iIntros "#HΨ1 #HΨ2". iModIntro. iIntros (v Φ) "Hprot".
+  iDestruct (protocol_agreement_sum_elim with "Hprot") as "[Hprot|Hprot]".
+  { iApply protocol_agreement_sum_intro_l. by iApply "HΨ1". }
+  { iApply protocol_agreement_sum_intro_r. by iApply "HΨ2". }
+Qed.
+
+Lemma iEff_le_marker f (Ψ1 Ψ2 : iEff Σ) : (Ψ1 ⊑ Ψ2 -∗ (f #> Ψ1) ⊑ (f #> Ψ2))%ieff.
+Proof.
+  iIntros "#HΨ". iModIntro. iIntros (v Φ) "Hprot".
+  iDestruct (protocol_agreement_marker_elim' with "Hprot") as (w) "[-> Hprot]".
+  iApply protocol_agreement_marker_intro. by iApply "HΨ".
+Qed.
+
+Lemma iEff_le_tele {TT1 TT2 TT1' TT2' : tele}
+  (v  : TT1  →        val) (P  : TT1  →        iProp Σ)
+  (w  : TT1  → TT2  → val) (Q  : TT1  → TT2  → iProp Σ)
+  (v' : TT1' →        val) (P' : TT1' →        iProp Σ)
+  (w' : TT1' → TT2' → val) (Q' : TT1' → TT2' → iProp Σ) :
+   ((>>.. x  >> ! (v  x   )  {{ P  x     }};
+     <<.. y  << ? (w  x  y)  {{ Q  x  y  }})
+      ⊑
+    (>>.. x' >> ! (v' x'   ) {{ P' x'    }};
+     <<.. y' << ? (w' x' y') {{ Q' x' y' }}))%ieff
+   ⊣⊢
+     □ (∀.. x,  P  x     -∗ (∃.. x', P' x'  ∗ ⌜ v x   = v' x'    ⌝ ∗
+       (∀.. y', Q' x' y' -∗ (∃.. y,  Q  x y ∗ ⌜ w x y = w' x' y' ⌝)))).
+Proof.
+  iSplit; iIntros "#Hle"; iModIntro.
+  - iIntros (x) "HP".
+    iSpecialize ("Hle" $! (v x) (<<..y<<?(w x y){{Q x y}})%ieff with "[HP]").
+    { iExists (<<..y<<?(w x y){{Q x y}})%ieff.
+      rewrite iEffPre_texist_eq iEffPre_base_eq.
+      iSplitL; [iExists x; iFrame|]; by auto. }
+    iDestruct "Hle" as (Φ) "[HP HQ]".
+    rewrite iEffPre_texist_eq iEffPre_base_eq.
+    iDestruct "HP" as (x') "[<- [HP HΦ]]". iExists x'. iFrame.
+    iSplit; [done|]. iIntros (y') "HQ'".
+    iSpecialize ("HΦ" $! (w' x' y') with "[HQ']").
+    { rewrite iEffPost_texist_eq iEffPost_base_eq. iExists y'. by iFrame. }
+    iSpecialize ("HQ" with "HΦ").
+    rewrite iEffPost_texist_eq iEffPost_base_eq.
+    iDestruct "HQ" as (y) "[<- HQ]". iExists y. by iFrame.
+  - iIntros (u Φ) "Hprot".
+    iDestruct "Hprot" as (Φ') "[HP HΦ']".
+    rewrite iEffPre_texist_eq iEffPre_base_eq.
+    iDestruct "HP" as (x) "[<- [HP HΦ]]".
+    iDestruct ("Hle" with "HP") as (x') "(HP' & -> & HQ)". iClear "Hle".
+    iExists (<<.. y<< ?(w x y){{ Q x y }})%ieff.
+    iSplitR "HΦ HΦ'".
+    { rewrite iEffPre_texist_eq. iExists x'. iFrame. iSplit; [done|].
+      iIntros (u') "HQ'". rewrite !iEffPost_texist_eq iEffPost_base_eq.
+      iDestruct "HQ'" as (y') "[<- HQ']".
+      iDestruct ("HQ" with "HQ'") as (y) "[HQ <-]".
+      iExists y. by iFrame. }
+    { iIntros (u) "HQ'". iApply "HΦ'". by iApply "HΦ". }
+Qed.
+
+End protocol_ordering.
+
+
+(** * Monotonicity. *)
+
+Section protocol_agreement_monotonicity.
+Context `{!irisG eff_lang Σ}.
+
+Lemma protocol_agreement_strong_mono v (Ψ1 Ψ2 : iEff Σ) Φ1 Φ2 :
+  (protocol_agreement v Ψ1 Φ1 -∗ Ψ1 ⊑ Ψ2 -∗ (∀ v, Φ1 v -∗ Φ2 v) -∗
+   protocol_agreement v Ψ2 Φ2)%ieff.
+Proof.
+  iIntros "Hprot_agr #HΨ HΦ". iApply "HΨ".
+  by iApply (protocol_agreement_mono with "Hprot_agr HΦ").
+Qed.
+
+End protocol_agreement_monotonicity.
