theories/scheduler.v
@@ -1,3 +1,9 @@
+(* scheduler.v
+
+   Verification of a asynchronous computation library implementation
+   that uses effects and handlers.
+*)
+
 From stdpp               Require Import list.
 From iris.proofmode      Require Import base tactics classes.
 From iris.algebra        Require Import excl_auth gset gmap agree.
@@ -9,346 +15,385 @@ From hazel               Require Import notation weakestpre deep_handler
 Section scheduler.
 Context `{!heapG Σ}.
 
-(**  Effects. *)
-
-(* Effect markers. *)
-
-Definition async : val → val := InjLV.
-Definition await : val → val := InjRV.
-
-(** Proof. *)
-
-(* Data structures. *)
+(* ************************************************************************** *)
+(** Data structures. *)
 
 Context {HList: ListLib Σ} {HQueue: QueueLib Σ}.
 
-(* Camera setup. We need the first cmra for the definition of [running_auth] and
-   [running_frang], and we need the second for the definition of [is_promise]
-   and [handler_inv]. *)
+
+(* ************************************************************************** *)
+(** Camera setup. *)
+
+(* The first camera is required for the definition of [running_auth]
+   and [running_frang] while the second is for the definition of
+   [is_promise], [promise_inv] and [ready]. *)
 
 Context `{!inG Σ (excl_authR boolO)}.
 Context `{!inG Σ (authR (gmapUR
                           (loc * gname)
                           (agreeR (laterO (val -d> (iPrePropO Σ))))))}.
 
-Context (promise_name : gname).
+
+(* ************************************************************************** *)
+(** Protocols. *)
+
+(* [is_promise p Φ] is the persistent proposition given to a thread after
+   an [async] effect. Any thread possesing this proposition can reclaim a
+   value [v] satisfying [□ Φ v]. *)
+
+Context (δ : gname).
 
 Definition promise_unfold (Φ : val → iProp Σ) :
-  agree (later (discrete_fun (λ (_ : val), iPrePropO Σ)))
-  :=
+  agree (later (discrete_fun (λ (_ : val), iPrePropO Σ))) :=
   to_agree (Next (λ v, iProp_unfold (Φ v))).
 
-(* [promise_inv γ p Φ] describes the invariant over the promise [p]: it is
-   either a reference to a value [v] satisfying [□ Φ v], or a reference to a
-   list of threads waiting for such a value [v]. The parameter [W_inv] is used
-   to specify threads waiting for the termination of a process associated with
-   a given promise. *)
+Definition is_promise p Φ := (∃ γ, own δ (◯ {[ (p, γ) := promise_unfold Φ ]}))%I.
 
-Definition running_auth γ (b : bool) := own γ (●E b).
-Definition running_frag γ (b : bool) := own γ (◯E b).
-Definition promise_inv γ p
-  (W_inv : (val -d> iPropO Σ) -d> (val -d> iPropO Σ))
-  (Φ : val -d> iPropO Σ) : iPropO Σ :=
-  (∃ b, running_auth γ b ∗ 
-    if b then
-      (∃ l ks, p ↦ InjRV l ∗ is_list l ks ∗ [∗ list] f ∈ ks, ▷ W_inv Φ f)
-    else
-      (∃ v, p ↦ InjLV v ∗ □ Φ v))%I.
+Global Instance is_promise_persistent p Φ : Persistent (is_promise p Φ).
+Proof. rewrite /ownI. apply _. Qed.
 
-(* [handler_inv W_inv] is the internal state of the handler. It enforces that
-   the set of created promises respect [promise_inv]. *)
+(*  Effects markers. *)
 
-Definition handler_inv W_inv :=
-  (∃ (S : gmap (loc * gname) (val → iProp Σ)),
-    own promise_name (● (promise_unfold <$> S : gmap _ _)) ∗
-    [∗ map] key ↦ Φ ∈ S, match key with (p, γ) => promise_inv γ p W_inv Φ end)%I.
+Definition async : val → val := InjLV.
+Definition await : val → val := InjRV.
 
-(* [is_promise' γ p Φ] is the persistent proposition given to a thread after an
-   [async] effect. Any thread possesing this proposition can reclaim a value [v]
-   satisfying [□ Φ v]. *)
+(* [Ψ_conc] is the protocol for concurrency effects (async and await).
+   It is defined as the fixpoint of [Ψ_conc_pre]. *)
 
-Definition is_promise' γ p Φ :=
-  own promise_name (◯ {[ (p, γ) := promise_unfold Φ ]}).
-Definition is_promise p Φ : iProp Σ := ∃ γ, is_promise' γ p Φ.
-
-(* [W_inv] is the specification of wainting threads. *)
-
-Definition W_inv_pre :
-  (val -d> (val -d> iPropO Σ) -d> (val -d> iPropO Σ) -d> (val -d> iPropO Σ)) →
-  (val -d> (val -d> iPropO Σ) -d> (val -d> iPropO Σ) -d> (val -d> iPropO Σ))
-  :=
-  (λ W_inv q Ready Φ f,
-    ∀ v, handler_inv (W_inv q Ready) -∗ (∃ n, is_queue q Ready n) -∗ □ Φ v -∗
-      EWP f v @ ∅ {{ _, True }})%I.
-
-Local Instance W_inv_pre_contractive : Contractive W_inv_pre.
-Proof.
-  rewrite /W_inv_pre=> n W_inv W_inv' HW q Ready Ψ f.
-  rewrite /handler_inv /promise_inv.
-  repeat (f_contractive || f_equiv); try apply HW.
-Qed.
-Definition W_inv_def : 
-   val -d> (val -d> iPropO Σ) -d> (val -d> iPropO Σ) -d> (val -d> iPropO Σ)
- :=
-  fixpoint W_inv_pre.
-Definition W_inv_aux : seal W_inv_def. Proof. by eexists. Qed.
-Definition W_inv := W_inv_aux.(unseal).
-Definition W_inv_eq : W_inv = W_inv_def := W_inv_aux.(seal_eq).
-Global Lemma W_inv_unfold q Ready Φ f :
-  W_inv q Ready Φ f ⊣⊢ W_inv_pre W_inv q Ready Φ f.
-Proof. rewrite W_inv_eq /W_inv_def. apply (fixpoint_unfold W_inv_pre). Qed.
-Global Instance W_inv_ne n :
-  Proper ((dist n) ==> (dist n) ==> (dist n) ==> (dist n) ==> (dist n)) W_inv.
-Proof.
-  induction (lt_wf n) as [n _ IH]=> q q' Hq Q Q' HQ Φ Φ' HΦ f f' Hf.
-  rewrite !W_inv_unfold /W_inv_pre /handler_inv /promise_inv.
-  do 3 f_equiv.
-  - do 20 f_equiv. f_contractive.
-    apply IH; try lia; eapply dist_le; eauto with lia.
-  - destruct Hq. destruct Hf. do 3 f_equiv; [| auto]; apply is_queue_ne; auto.
-Qed.
-Global Instance W_inv_proper : Proper ((≡) ==> (≡) ==> (≡) ==> (≡) ==> (≡)) W_inv.
-Proof. intros ????????????. apply equiv_dist=>n. by apply W_inv_ne; apply equiv_dist. Qed.
-
-(* [Ready] is the specification of paused threads that were put in the queue. *)
-
-Definition Ready_pre q : (val -d> iPropO Σ) → (val -d> iPropO Σ)
-  :=
-  (λ Ready e, handler_inv (W_inv q Ready) -∗ (∃ n, ▷ is_queue q Ready n) -∗
-      EWP e #() @ ∅ {{ _, True }})%I.
-
-Local Instance Ready_pre_contractive q : Contractive (Ready_pre q).
-Proof.
-  rewrite /Ready_pre=> n Ready Ready' HQ e.
-  rewrite /handler_inv /promise_inv.
-  repeat (f_contractive || apply is_queue_ne || f_equiv); done.
-Qed.
-
-Definition Ready_def q : (val -d> iPropO Σ) := fixpoint (Ready_pre q).
-Definition Ready_aux : seal Ready_def. Proof. by eexists. Qed.
-Definition Ready := Ready_aux.(unseal).
-Definition Ready_eq : Ready = Ready_def := Ready_aux.(seal_eq).
-Global Lemma Ready_unfold q e : Ready q e ⊣⊢ Ready_pre q (Ready q) e.
-Proof. rewrite Ready_eq /Ready_def. apply (fixpoint_unfold (Ready_pre q)). Qed.
-Global Instance Ready_ne q n : Proper ((dist n) ==> (dist n)) (Ready q).
-Proof. solve_proper. Qed.
-Global Instance Ready_proper q : Proper ((≡) ==> (≡)) (Ready q).
-Proof. solve_proper. Qed.
-
-(* [Ψ_concurrency] is the protocol for concurrency effects (async and await).
-   It is defined as the fixpoint of [Ψ_concurrency_pre]. *)
-
-Definition Ψ_concurrency_pre : iEff Σ → iEff Σ := (λ Ψ,
-
-    (async #> (>> e Φ >> !  (e)       {{ ▷ EWP e #() @ ∅ <| Ψ |> {{ v, □ Φ v }} }};
-               << p   << ? #(p : loc) {{ is_promise p Φ                         }}))
+Definition Ψ_conc_pre : iEff Σ → iEff Σ := (λ Ψ,
+    (async #> (>> e Φ >> !  (e)       {{ ▷ EWP e #() <| Ψ |> {{ v, □ Φ v }} }};
+               << p   << ? #(p : loc) {{ is_promise p Φ                     }}))
       <+>
-
     (await #> (>> p Φ >> ! #(p : loc) {{ is_promise p Φ }};
                << v   << ?  (v)       {{ □ Φ v          }})))%ieff.
 
 
-Local Instance Ψ_concurrecy_pre_contractive : Contractive (Ψ_concurrency_pre).
-Proof. rewrite /Ψ_concurrency_pre=> n Ψ Ψ' HΨ.
+Local Instance Ψ_conc_pre_contractive : Contractive (Ψ_conc_pre).
+Proof. rewrite /Ψ_conc_pre=> n Ψ Ψ' HΨ.
        by repeat (apply ewp_ne||apply iEffPre_base_ne||f_contractive||f_equiv).
 Qed.
-Definition Ψ_concurrency_def : iEff Σ := fixpoint (Ψ_concurrency_pre).
-Definition Ψ_concurrency_aux : seal Ψ_concurrency_def. Proof. by eexists. Qed.
-Definition Ψ_concurrency := Ψ_concurrency_aux.(unseal).
-Definition Ψ_concurrency_eq : Ψ_concurrency = Ψ_concurrency_def :=
-  Ψ_concurrency_aux.(seal_eq).
-Global Lemma Ψ_concurrency_unfold : Ψ_concurrency ≡ Ψ_concurrency_pre (Ψ_concurrency).
-Proof. rewrite Ψ_concurrency_eq /Ψ_concurrency_def.
-       by apply (fixpoint_unfold (Ψ_concurrency_pre)).
+Definition Ψ_conc_def : iEff Σ := fixpoint (Ψ_conc_pre).
+Definition Ψ_conc_aux : seal Ψ_conc_def. Proof. by eexists. Qed.
+Definition Ψ_conc := Ψ_conc_aux.(unseal).
+Definition Ψ_conc_eq : Ψ_conc = Ψ_conc_def := Ψ_conc_aux.(seal_eq).
+Global Lemma Ψ_conc_unfold : Ψ_conc ≡ Ψ_conc_pre (Ψ_conc).
+Proof. rewrite Ψ_conc_eq /Ψ_conc_def.
+       by apply (fixpoint_unfold (Ψ_conc_pre)).
 Qed.
 
-Definition Ψ_async : iEff Σ :=
-  (async #>
-    (>> e Φ       >> !  e {{ ▷ EWP e #() @ ∅ <|Ψ_concurrency|> {{v, □ Φ v}} }};
-     << (p : loc) << ? #p {{ is_promise p Φ                                 }})).
+(* Properties of the protocol [Ψ_conc]. *)
 
-Definition Ψ_await : iEff Σ :=
-  (await #>
-    (>> p Φ >> ! #(p : loc) {{ is_promise p Φ }};
-     << v   << ?   v        {{ □ Φ v          }})).
+Section Ψ_conc.
 
-Lemma Ψ_concurrency_eq_sum : (Ψ_concurrency ≡ Ψ_async <+> Ψ_await)%ieff.
-Proof. by rewrite Ψ_concurrency_unfold. Qed.
+  Definition Ψ_async : iEff Σ :=
+    (async #> (>> e Φ >> !  (e)       {{ ▷ EWP e #() <|Ψ_conc|> {{v, □ Φ v}} }};
+               << p   << ? #(p : loc) {{ is_promise p Φ                      }})).
+  Definition Ψ_await : iEff Σ :=
+    (await #> (>> p Φ >> ! #(p : loc) {{ is_promise p Φ }};
+               << v   << ?   v        {{ □ Φ v          }})).
 
-Lemma Ψ_concurrency_agreement E v Φ' :
-  protocol_agreement E v Ψ_concurrency Φ' ⊢
-    ((protocol_agreement E v Ψ_async Φ') ∨ (protocol_agreement E v Ψ_await Φ')).
+  Lemma Ψ_conc_eq_sum : (Ψ_conc ≡ Ψ_async <+> Ψ_await)%ieff.
+  Proof. by rewrite Ψ_conc_unfold. Qed.
+
+  Lemma Ψ_conc_agreement v Φ' :
+    protocol_agreement v Ψ_conc Φ' ⊣⊢ ((protocol_agreement v Ψ_async Φ') ∨
+                                       (protocol_agreement v Ψ_await Φ')).
+  Proof.
+    rewrite Ψ_conc_eq_sum. iSplit; iIntros "Hprot_agr".
+    - iDestruct (protocol_agreement_sum_elim with "Hprot_agr") as "[H|H]"; by eauto.
+    - iDestruct "Hprot_agr" as "[H|H]"; [
+      by iApply protocol_agreement_sum_intro_l |
+      by iApply protocol_agreement_sum_intro_r ].
+  Qed.
+  Lemma Ψ_async_agreement v Φ' : protocol_agreement v Ψ_async Φ' ≡
+    (∃ e Φ, ⌜ v = async e ⌝ ∗ (▷ EWP e #() <| Ψ_conc |> {{ v, □ Φ v }}) ∗
+          (∀ (p : loc), is_promise p Φ -∗ Φ' #p))%I.
+  Proof.
+    rewrite /Ψ_async (iEff_marker_tele' [tele _ _] [tele _]).
+    rewrite (protocol_agreement_tele' [tele _ _] [tele _]). by auto.
+  Qed.
+  Lemma Ψ_await_agreement v Φ' : protocol_agreement v Ψ_await Φ' ≡
+    (∃ (p : loc) Φ, ⌜ v = await #p ⌝ ∗ is_promise p Φ ∗
+        (∀ v, □ Φ v -∗ Φ' v))%I.
+  Proof.
+    rewrite /Ψ_await (iEff_marker_tele' [tele _ _] [tele _]) //=.
+    rewrite (protocol_agreement_tele' [tele _ _] [tele _]). by auto.
+  Qed.
+
+End Ψ_conc.
+
+(* Properties of [promise_unfold] and [is_promise]. *)
+
+Section promise_unfold.
+
+  Lemma promise_lookup (S : gmap (loc * gname) (val → iProp Σ)) γ p Φ :
+    own δ (● (promise_unfold <$> S : gmap _ _)) ∗
+    own δ (◯ {[(p, γ) := promise_unfold Φ]}) ⊢
+    ∃ Ψ, ⌜ S !! (p, γ) = Some Ψ ⌝ ∗ (promise_unfold Ψ ≡ promise_unfold Φ).
+  Proof.
+    rewrite -own_op own_valid auth_both_validI /=.
+    iIntros "[_ [#HS #HvS]]". iDestruct "HS" as (S') "HS".
+    rewrite gmap_equivI gmap_validI.
+    iSpecialize ("HS" $! (p, γ)). iSpecialize ("HvS" $! (p, γ)).
+    rewrite lookup_fmap lookup_op lookup_singleton.
+    rewrite option_equivI.
+    case: (S  !! (p, γ))=> [Ψ|] /=; [|
+    case: (S' !! (p, γ))=> [Ψ'|] /=; by iExFalso].
+    iExists Ψ. iSplit; first done.
+    case: (S' !! (p, γ))=> [Ψ'|] //=.
+    iRewrite "HS" in "HvS". rewrite uPred.option_validI agree_validI.
+    iRewrite -"HvS" in "HS". by rewrite agree_idemp.
+  Qed.
+
+  Lemma promise_unfold_equiv (Ψ Φ : val → iProp Σ) :
+    promise_unfold Ψ ≡ promise_unfold Φ -∗ ▷ (∀ v, Ψ v ≡ Φ v : iProp Σ).
+  Proof.
+    rewrite /promise_unfold.
+    rewrite agree_equivI. iIntros "Heq". iNext. iIntros (v).
+    iDestruct (discrete_fun_equivI with "Heq") as "Heq".
+    iSpecialize ("Heq" $! v).
+    by iApply iProp_unfold_equivI.  
+  Qed.
+
+End promise_unfold.
+
+
+(* ************************************************************************** *)
+(** Proof Invariants. *)
+
+Definition running_auth γ (b : bool) := own γ (●E b).
+Definition running_frag γ (b : bool) := own γ (◯E b).
+
+(* Properties of [running_auth] and [running_frag]. *)
+
+Section running.
+
+  Lemma running_auth_twice γ b b' : (running_auth γ b ∗ running_auth γ b') ⊢ False.
+  Proof.
+    rewrite /running_auth -own_op own_valid. iIntros "#H".
+    iAssert (⌜ Excl' b = Excl' b' ⌝)%I as "%"; iRevert "H".
+    { iIntros (H). iPureIntro. by apply (auth_auth_frac_op_invL _ _ _ _ H). }
+    inversion H. rewrite -auth_auth_frac_op auth_validI. by iIntros "#[% _]".
+  Qed.
+  Lemma running_frag_twice γ b b' : running_frag γ b ∗ running_frag γ b' ⊢ False.
+  Proof.
+    rewrite /running_frag -own_op own_valid.
+    iIntros (H). by destruct (excl_auth_frag_valid_op_1_l _ _ H).
+  Qed.
+  Lemma running_agree γ b b' : ⊢ running_auth γ b ∗ running_frag γ b' → ⌜ b = b' ⌝.
+  Proof. iIntros "[H● H◯]". by iDestruct (own_valid_2 with "H● H◯") as %?%excl_auth_agreeL. Qed.
+  Lemma running_agree' γ b b' : b ≠ b' → running_auth γ b -∗ running_frag γ b' -∗ False.
+  Proof.
+    iIntros (Hneq) "H● H◯".
+    by iDestruct (running_agree γ b b' with "[H● H◯]") as "->"; iFrame.
+  Qed.
+  Lemma running_upd γ b1 b1' b2 : 
+    running_auth γ b1 -∗ running_frag γ b1' ==∗ running_auth γ b2  ∗ running_frag γ b2.
+  Proof.
+    iIntros "H● H◯".
+    iMod (own_update_2 _ _ _ (●E b2 ⋅ ◯E (b2 : ofe_car boolO)) with "H● H◯") as "[$$]".
+    { by apply excl_auth_update. } { done. }
+  Qed.
+
+End running.
+
+(* [promise_inv] is the main proof invariant. It asserts the existence of a
+   set of promises, each of which has either already been fulfilled or not.
+   If not, a number of threads might be waiting for this event to happen. *)
+
+Definition promise_inv_pre :
+  (val -d> (val -d> iPropO Σ) -d> iPropO Σ) →
+  (val -d> (val -d> iPropO Σ) -d> iPropO Σ)
+  := λ promise_inv q ready,
+  (∃ (S : gmap (loc * gname) (val → iProp Σ)),
+   own δ (● (promise_unfold <$> S : gmap _ _)) ∗
+   [∗ map] key ↦ Φ ∈ S,
+   match key with (p, γ) =>
+     ∃ b, running_auth γ b ∗ 
+     match b with
+     | false =>
+        ∃ v, p ↦ InjLV v ∗ □ Φ v
+     | true =>
+        ∃ l ks, p ↦ InjRV l ∗ is_list l ks ∗
+          [∗ list] k ∈ ks,
+            ∀ (v : val), □ Φ v -∗
+              ▷ (promise_inv q ready) -∗
+                ▷ (∃ (n : nat), is_queue q ready n) -∗
+                  EWP (k : val) v {{ _, True }}
+     end
+    end)%I.
+
+Local Instance promise_inv_pre_contractive : Contractive promise_inv_pre.
 Proof.
-  iIntros "Hprot_agr". rewrite Ψ_concurrency_eq_sum.
-  iDestruct (protocol_agreement_sum_elim with "Hprot_agr") as "[H|H]"; by eauto.
+  rewrite /promise_inv_pre=> n promise_inv promise_inv' HW q ready.
+  repeat (f_contractive || f_equiv); try apply HW.
+Qed.
+Definition promise_inv_def := fixpoint promise_inv_pre.
+Definition promise_inv_aux : seal promise_inv_def. Proof. by eexists. Qed.
+Definition promise_inv := promise_inv_aux.(unseal).
+Definition promise_inv_eq : promise_inv = promise_inv_def :=
+  promise_inv_aux.(seal_eq).
+Global Lemma promise_inv_unfold q ready :
+  promise_inv q ready ⊣⊢ promise_inv_pre promise_inv q ready.
+Proof. rewrite promise_inv_eq /promise_inv_def.
+       apply (fixpoint_unfold promise_inv_pre).
+Qed.
+Global Instance promise_inv_ne n :
+  Proper ((dist n) ==> (dist n) ==> (dist n)) promise_inv.
+Proof.
+  induction (lt_wf n) as [n _ IH]=> q q' Hq ready ready' Hready.
+  inversion Hq. rewrite !promise_inv_unfold /promise_inv_pre.
+  repeat (f_contractive || apply promise_inv_ne || apply is_queue_ne
+         ||    apply IH || f_equiv);
+  try lia; by (eapply dist_le; eauto with lia).
+Qed.
+Global Instance promise_inv_proper : Proper ((≡) ==> (≡) ==> (≡)) promise_inv.
+Proof. intros ??????. apply equiv_dist=>n.
+       by apply promise_inv_ne; apply equiv_dist.
 Qed.
 
-Lemma Ψ_async_agreement E v Φ' :
-  protocol_agreement E v Ψ_async Φ' ≡
-    (|={E,∅}=>
-       ∃ e Φ, ⌜ v = async e ⌝ ∗ (▷ EWP e #() @ ∅ <|Ψ_concurrency|> {{v, □ Φ v}}) ∗
-          (∀ (p : loc), is_promise p Φ ={∅,E}=∗ Φ' #p))%I.
+(* Properties of [promise_inv]. *)
+
+Section promise_inv.
+  Context (q : val) (ready : val -d> iPropO Σ).
+
+  Definition points_to p γ Φ : iProp Σ :=
+   ∃ b, running_auth γ b ∗ 
+   match b with
+   | false =>
+      ∃ v, p ↦ InjLV v ∗ □ Φ v
+   | true =>
+      ∃ l ks, p ↦ InjRV l ∗ is_list l ks ∗
+        [∗ list] k ∈ ks,
+          ∀ (v : val), □ Φ v -∗
+            ▷ (promise_inv q ready) -∗
+              ▷ (∃ (n : nat), is_queue q ready n) -∗
+                EWP (k : val) v {{ _, True }}
+   end.
+
+  Lemma promise_alloc Φ :
+    ⊢ EWP ref (InjR (list_nil #())) {{ p',
+        ∃ (p : loc) γ, ⌜ p' = #p ⌝ ∗ running_frag γ true ∗ points_to p γ Φ }}.
+  Proof.
+    iApply (ewp_bind (ConsCtx AllocCtx (ConsCtx InjRCtx EmptyCtx))). done.
+    iApply ewp_mono; [|iApply list_nil_spec].
+    iIntros (l) "Hlist". iModIntro.
+    iApply (Ectxi_ewp_bind AllocCtx). done.
+    iApply ewp_pure_step. apply pure_prim_step_InjR.
+    iApply ewp_value. simpl.
+    iApply ewp_mono'. { by iApply (ewp_alloc _ (InjRV l)). }
+    iIntros (v) "Hp". iDestruct "Hp" as (p) "[-> Hp]".
+    iMod (own_alloc (●E true ⋅ ◯E true)) as (γ) "[Hauth Hfrag]".
+    - by apply excl_auth_valid.
+    - iModIntro. iExists p, γ. iFrame. iSplit; first auto.
+      iExists true. iFrame. iExists l, []. by iFrame.
+  Qed.
+
+  Lemma promise_upd p γ Φ :
+    promise_inv q ready ∗ points_to p γ Φ ==∗
+    promise_inv q ready ∗ own δ (◯ {[ (p, γ) := promise_unfold Φ ]}).
+  Proof.
+    iIntros "[Hpromise_inv Hpoints_to]". rewrite {1}promise_inv_unfold.
+    iDestruct "Hpromise_inv" as (S) "[HS Hinv]".
+    destruct (S !! (p, γ)) as [Ψ|] eqn:Heq.
+    - rewrite (big_opM_delete _ _ _ _ Heq).
+      iDestruct "Hinv" as "[Hpoints_to' _]".
+      iDestruct "Hpoints_to'" as (b') "[Hrunning' _]".
+      iDestruct "Hpoints_to"  as (b)  "[Hrunning  _]".
+      by iDestruct (running_auth_twice with "[Hrunning' Hrunning]") as "H"; iFrame.
+    - iMod (own_update with "HS") as "[HS HiP]".
+      { apply (@auth_update_alloc (gmapUR _ _) (promise_unfold <$> S)).
+        apply (alloc_singleton_local_update _ (p, γ) (promise_unfold Φ)).
+        by rewrite /= lookup_fmap Heq. done. }
+      iModIntro. iFrame.
+      rewrite {-1}promise_inv_unfold. iExists (<[(p, γ):= Φ]> S).
+      rewrite /= fmap_insert. iFrame.
+      rewrite big_opM_insert. iFrame. done.
+  Qed.
+
+  Lemma promise_agree p γ Φ :
+    promise_inv q ready ∗
+    own δ (◯ {[(p, γ) := promise_unfold Φ]}) -∗
+    (∃ S, own δ (● (promise_unfold <$> S : gmap _ _)) ∗
+      ([∗ map] key ↦ Φ ∈ delete (p, γ) S,
+          match key with (p, γ) => points_to p γ Φ end) ∗
+        (∃ Ψ, ⌜ S !! (p, γ) = Some Ψ ⌝ ∗ points_to p γ Ψ ∗
+          (promise_unfold Ψ ≡ promise_unfold Φ))).
+  Proof.
+    iIntros "[Hpromise_inv Hpoints_to]". rewrite promise_inv_unfold.
+    iDestruct "Hpromise_inv" as (S) "[HS Hinv]".
+    iDestruct (promise_lookup S γ p Φ with "[$]") as (Ψ Hlookup) "#Heq".
+    iDestruct (big_sepM_delete _ _ (p, γ) with "Hinv") as "[Hpromise_inv Hinv]".
+    eauto. iExists S. iFrame. iExists Ψ. iFrame. by iSplit; first auto.
+  Qed.
+
+End promise_inv.
+
+(* [ready] is the specification satisfied by paused threads. *)
+
+Definition ready_pre : (val -d> val -d> iPropO Σ) → (val -d> val -d> iPropO Σ)
+  := λ ready q k,
+  (▷ (promise_inv q (ready q)) -∗
+     ▷ (∃ (n : nat), is_queue q (ready q) n) -∗
+       EWP (k : val) #() {{ _, True }})%I.
+
+Local Instance ready_pre_contractive : Contractive ready_pre.
 Proof.
-  rewrite /Ψ_async (iEff_marker_tele' [tele _ _] [tele _]).
-  rewrite (protocol_agreement_tele' [tele _ _] [tele _]). by auto.
+  rewrite /ready_pre=> n ready ready' HW q k.
+  repeat (f_contractive || apply promise_inv_ne || apply is_queue_ne || f_equiv);
+  by try (eapply dist_le; eauto with lia).
+Qed.
+Definition ready_def := fixpoint ready_pre.
+Definition ready_aux : seal ready_def. Proof. by eexists. Qed.
+Definition ready := ready_aux.(unseal).
+Definition ready_eq : ready = ready_def := ready_aux.(seal_eq).
+Global Lemma ready_unfold q k : ready q k ⊣⊢ ready_pre ready q k.
+Proof. rewrite ready_eq /ready_def.
+       apply (fixpoint_unfold ready_pre).
+Qed.
+Global Instance ready_ne n : Proper ((dist n) ==> (dist n) ==> (dist n)) ready.
+Proof.
+  induction (lt_wf n) as [n _ IH]=> q q' Hq k k' Hk.
+  rewrite !ready_unfold /ready_pre.
+  repeat (f_contractive || apply promise_inv_ne || apply is_queue_ne || f_equiv);
+  by try (eapply dist_le; eauto with lia).
+Qed.
+Global Instance ready_inv_proper : Proper ((≡) ==> (≡) ==> (≡)) promise_inv.
+Proof. intros ??????. apply equiv_dist=>n.
+       by apply promise_inv_ne; apply equiv_dist.
 Qed.
 
-Lemma Ψ_await_agreement E v Φ' :
-  protocol_agreement E v Ψ_await Φ' ≡
-    (|={E,∅}=>
-       ∃ (p : loc) Φ, ⌜ v = await #p ⌝ ∗ is_promise p Φ ∗
-          (∀ v, □ Φ v ={∅,E}=∗ Φ' v))%I.
+
+(* ************************************************************************** *)
+(** Verification of the Library. *)
+
+Lemma ewp_async (e : val) Φ :
+  EWP e #() <| Ψ_conc |> {{ v, □ Φ v }} ⊢
+    EWP do: (async e) <| Ψ_conc |>
+      {{ p', ∃ (p : loc), ⌜ p' = #p ⌝ ∗ is_promise p Φ }}.
 Proof.
-  rewrite /Ψ_await (iEff_marker_tele' [tele _ _] [tele _]).
-  rewrite (protocol_agreement_tele' [tele _ _] [tele _]). by auto.
+  iIntros "He".
+  iApply ewp_pure_step. apply pure_prim_step_do.
+  iApply ewp_eff. rewrite Ψ_conc_agreement Ψ_async_agreement.
+  iLeft. iExists e, Φ. iSplit; [done|]. iFrame.
+  iIntros (p) "Hp". iApply ewp_value. iExists p. by iFrame.
 Qed.
 
-(* Auxiliary lemmas. *)
-
-Local Instance promise_inv_ne γ p q n :
-  Proper ((dist n) ==> (dist n)) (promise_inv γ p (W_inv q (Ready q))).
+Lemma ewp_await (p : loc) Φ :
+  is_promise p Φ ⊢ EWP do: (await #p) <| Ψ_conc |> {{ v, □ Φ v }}.
 Proof.
-  intros ???. rewrite /promise_inv.
-  do 8 f_equiv; last eauto. solve_proper.
-Qed.
-
-Local Instance promise_inv_proper γ p q :
-  Proper ((≡) ==> (≡)) (promise_inv γ p (W_inv q (Ready q))).
-Proof. intros ???. apply equiv_dist=>n. by apply promise_inv_ne, equiv_dist. Qed.
-
-Lemma running_auth_twice γ b b' : running_auth γ b ∗ running_auth γ b' ⊢ False.
-Proof.
-  rewrite /running_auth. rewrite -own_op own_valid.
-  case (bool_dec b b').
-  + intros ->. rewrite -auth_auth_frac_op auth_validI. by iIntros ([? _]).
-  + iIntros (Heq' Hvalid).
-    cut (b = b'); [done|].
-    cut (Some (Excl b) = Some (Excl b')). naive_solver.
-    by apply (auth_auth_frac_op_invL _ _ _ _ Hvalid).
-Qed.
-
-Lemma running_frag_twice γ b b' : running_frag γ b ∗ running_frag γ b' ⊢ False.
-Proof.
-  rewrite /running_frag. rewrite -own_op own_valid.
-  iIntros (Hvalid). by destruct (excl_auth_frag_valid_op_1_l _ _ Hvalid).
-Qed.
-
-Lemma running_agree γ b b' : ⊢ running_auth γ b ∗ running_frag γ b' → ⌜ b = b' ⌝.
-Proof.
-  iIntros "[H● H◯]". by iDestruct (own_valid_2 with "H● H◯") as %?%excl_auth_agreeL.
-Qed.
-
-Lemma running_agree' γ b b' : 
-  b ≠ b' → running_auth γ b -∗ running_frag γ b' -∗ False.
-Proof.
-  intros Hneq. iIntros "Hauth Hfrag".
-  iPoseProof (running_agree with "[Hauth Hfrag]") as "%". by iFrame. done.
-Qed.
-
-Lemma running_upd γ b1 b2 b : 
-  running_auth γ b1 -∗ running_frag γ b2 ==∗
-  running_auth γ b   ∗ running_frag γ b.
-Proof.
-  iIntros "Hγ● Hγ◯".
-  iMod (own_update_2 _ _ _ (●E (b : ofe_car boolO) ⋅ ◯E (b : ofe_car boolO))
-    with "Hγ● Hγ◯") as "[$$]".
-  { by apply excl_auth_update. }
-  done.
-Qed.
-
-Instance is_promise_persistent γ p Φ : Persistent (is_promise' γ p Φ).
-Proof. rewrite /ownI. apply _. Qed.
-
-Lemma promise_alloc E Φ W_inv :
-  ⊢ EWP ref (InjR (list_nil #())) @ E
-      {{ v, ∃ (p : loc) γ, ⌜ v = #p ⌝ ∗ running_frag γ true ∗ promise_inv γ p Φ W_inv }}.
-Proof.
-  iApply (ewp_bind (ConsCtx AllocCtx (ConsCtx InjRCtx EmptyCtx))). done.
-  iApply ewp_mono; [|iApply list_nil_spec].
-  iIntros (l) "Hlist". iModIntro.
-  iApply (Ectxi_ewp_bind AllocCtx). done.
-  iApply ewp_pure_step. apply pure_prim_step_InjR.
-  iApply ewp_value. simpl.
-  iApply ewp_mono'. { by iApply (ewp_alloc E (InjRV l)). }
-  iIntros (v) "Hp". iDestruct "Hp" as (p) "[-> Hp]".
-  iMod (own_alloc (●E true ⋅ ◯E true)) as (γ) "[Hauth Hfrag]".
-  - by apply excl_auth_valid.
-  - iModIntro. iExists p, γ. iFrame. iSplit; first auto.
-    iExists true. iFrame. iExists l, []. by iFrame.
-Qed.
-
-Lemma promise_upd γ p W_inv Φ :
-  handler_inv W_inv ∗ promise_inv γ p W_inv Φ ==∗
-  handler_inv W_inv ∗ is_promise' γ p Φ.
-Proof.
-  iIntros "[Hhandler_inv Hpromise]".
-  iDestruct "Hhandler_inv" as (S) "[HS Hinv]".
-  destruct (S !! (p, γ)) as [Ψ|] eqn:Heq.
-  - rewrite (big_opM_delete _ _ _ _ Heq).
-    iDestruct "Hinv" as "[Hpromise' _]".
-    iDestruct "Hpromise'" as (b') "[Hrunning' _]".
-    iDestruct "Hpromise"  as (b)  "[Hrunning  _]".
-    by iDestruct (running_auth_twice with "[Hrunning' Hrunning]") as "H"; iFrame.
-  - iMod (own_update with "HS") as "[HS HiP]".
-    { apply (@auth_update_alloc (gmapUR _ _) (promise_unfold <$> S)).
-      apply (alloc_singleton_local_update _ (p, γ) (promise_unfold Φ)).
-      by rewrite /= lookup_fmap Heq. done. }
-    iModIntro. iFrame. iExists (<[(p, γ):= Φ]> S).
-    rewrite /= fmap_insert. iFrame.
-    rewrite big_opM_insert. iFrame. done.
-Qed.
-
-Lemma promise_lookup (S : gmap (loc * gname) (val → iProp Σ)) γ p Φ :
-  own promise_name (● (promise_unfold <$> S : gmap _ _)) ∗
-  own promise_name (◯ {[(p, γ) := promise_unfold Φ]}) ⊢
-  ∃ Ψ, ⌜ S !! (p, γ) = Some Ψ ⌝ ∗ (promise_unfold Ψ ≡ promise_unfold Φ).
-Proof.
-  rewrite -own_op own_valid auth_both_validI /=.
-  iIntros "[_ [#HS #HvS]]". iDestruct "HS" as (S') "HS".
-  rewrite gmap_equivI gmap_validI.
-  iSpecialize ("HS" $! (p, γ)). iSpecialize ("HvS" $! (p, γ)).
-  rewrite lookup_fmap lookup_op lookup_singleton.
-  rewrite option_equivI.
-  case: (S  !! (p, γ))=> [Ψ|] /=; [|
-  case: (S' !! (p, γ))=> [Ψ'|] /=; by iExFalso].
-  iExists Ψ. iSplit; first done.
-  case: (S' !! (p, γ))=> [Ψ'|] //=.
-  iRewrite "HS" in "HvS". rewrite uPred.option_validI agree_validI.
-  iRewrite -"HvS" in "HS". by rewrite agree_idemp.
-Qed.
-
-Lemma promise_unfold_equiv (Ψ Φ : val → iProp Σ) :
-  promise_unfold Ψ ≡ promise_unfold Φ -∗ ▷ (∀ v, Ψ v ≡ Φ v : iProp Σ).
-Proof.
-  rewrite /promise_unfold.
-  rewrite agree_equivI. iIntros "Heq". iNext. iIntros (v).
-  iDestruct (discrete_fun_equivI with "Heq") as "Heq".
-  iSpecialize ("Heq" $! v).
-  by iApply iProp_unfold_equivI.  
-Qed.
-
-Lemma promise_agree γ p W_inv Φ :
-  handler_inv W_inv ∗ is_promise' γ p Φ -∗
-  (∃ S, own promise_name (● (promise_unfold <$> S : gmap _ _)) ∗
-    ([∗ map] key ↦ Φ ∈ delete (p, γ) S,
-        match key with (p, γ) => promise_inv γ p W_inv Φ end) ∗
-      (∃ Ψ, ⌜ S !! (p, γ) = Some Ψ ⌝ ∗ promise_inv γ p W_inv Ψ ∗
-        (promise_unfold Ψ ≡ promise_unfold Φ))).
-Proof.
-  iIntros "[Hhandler_inv Hpromise]".
-  iDestruct "Hhandler_inv" as (S) "[HS Hinv]".
-  rewrite /is_promise.
-  iDestruct (promise_lookup S γ p Φ with "[$]") as (Ψ Hlookup) "#Heq".
-  iDestruct (big_sepM_delete _ _ (p, γ) with "Hinv") as "[Hpromise_inv Hinv]".
-  eauto. iExists S. iFrame. iExists Ψ. iFrame. by iSplit; first auto.
+  iIntros "Hp".
+  iApply ewp_pure_step. apply pure_prim_step_do.
+  iApply ewp_eff. rewrite Ψ_conc_agreement Ψ_await_agreement.
+  iRight. iExists p, Φ. iSplit; [done|]. iFrame.
+  iIntros (v) "#HΦ". by iApply ewp_value.
 Qed.
 
 Definition run : val := λ: "main",
   let: "q" := queue_create #() in
 
-  let: "run_next" := λ: <>,
-    if: queue_empty "q" then #() else
-      (queue_pop "q") #()
+  let: "next" := λ: <>,
+    if: queue_empty "q" then #() else (queue_pop "q") #()
   in
 
   let: "fulfill" := rec: "fulfill" "p" "e" :=
@@ -365,15 +410,15 @@ Definition run : val := λ: "main",
             match: Load "p" with
               InjL "v"  => "k" "v"
             | InjR "ks" =>
-                "p" <- InjR (list_cons (λ: "x", "k" "x") "ks");;
-                "run_next" #()
+                "p" <- InjR (list_cons "k" "ks");;
+                "next" #()
             end
         end)
     | return (λ: "v",
         match: Load "p" with InjL <> => #() | InjR "ks" =>
           list_iter (λ: "k", queue_push "q" (λ: <>, "k" "v")) "ks";;
           "p" <- InjL "v";;
-          "run_next" #()
+          "next" #()
         end)
     end
   in
@@ -381,32 +426,33 @@ Definition run : val := λ: "main",
   "fulfill" (ref (InjR (list_nil #()))) "main".
 
 Lemma run_spec' (main : val) Φ :
-  (∀ W_inv, handler_inv W_inv) -∗
-    EWP main #() @ ∅ <| Ψ_concurrency |> {{ v, □ Φ v }} -∗
-      EWP run main @ ∅ {{ _, True }}.
+  (∀ q ready, promise_inv q ready) -∗
+    EWP main #() <| Ψ_conc |> {{ v, □ Φ v }} -∗
+      EWP run main {{ _, True }}.
 Proof.
-  iIntros "Hhandler Hmain". unfold run.
+  iIntros "Hpromise_inv Hmain".
   iApply ewp_pure_step. apply pure_prim_step_beta. simpl.
   iApply (Ectxi_ewp_bind (AppRCtx _)). done.
   iApply ewp_strong_mono; first done; [
   iApply queue_create_spec | iApply iEff_le_refl |].
-  iIntros (q) "Hq". iSpecialize ("Hq" $! (Ready q)).
-  iSpecialize ("Hhandler" $! (W_inv q (Ready q))).
+  iIntros (q) "Hq". iSpecialize ("Hq" $! (ready q)).
+  iSpecialize ("Hpromise_inv" $! q (ready q)).
 
-  (* ************************************************************************ *)
-  (** Verification of [run_next]. *)
+  (* ************************************************************** *)
+  (** Verification of [next]. *)
 
   (* Specification. *)
-  iAssert (□ (∀ n, handler_inv (W_inv q (Ready q)) -∗ is_queue q (Ready q) n -∗
+  iAssert (∀ q, □ (▷ promise_inv q (ready q) -∗ ▷ (∃ n, is_queue q (ready q) n) -∗
     EWP
-      (λ: <>, if: queue_empty q then #() else queue_pop q #())%V #() @ ∅
+      (λ: <>, if: queue_empty q then #() else queue_pop q #())%V #()
     {{ _, True }}))%I
-  as "#run_next_spec".
+  as "#next_spec".
 
   (* Proof. *)
-  { iModIntro. iIntros (n) "Hhandler_inv Hq".
-    iApply ewp_pure_step. apply pure_prim_step_beta. simpl.
+  { iIntros (q'). iModIntro. iIntros "Hpromise_inv Hq".
+    iApply ewp_pure_step'. apply pure_prim_step_beta. simpl. iNext.
     iApply (Ectxi_ewp_bind (IfCtx _ _)). done.
+    iDestruct "Hq" as (n) "Hq".
     iApply (ewp_mono' with "[Hq]"); [
     iApply (queue_empty_spec with "Hq") |].
     simpl. case n.
@@ -419,12 +465,12 @@ Proof.
       iApply (ewp_mono' with "[Hq]");  [
       iApply (queue_pop_spec with "Hq")|].
       simpl. iModIntro. iIntros (k) "[Hq Hk]".
-      rewrite !Ready_unfold /Ready_pre.
-      iApply (ewp_mono' with "[Hk Hhandler_inv Hq]").
-      { iApply ("Hk" with "Hhandler_inv"). iExists m. by iFrame. }
+      rewrite !ready_unfold /ready_pre.
+      iApply (ewp_mono' with "[Hk Hpromise_inv Hq]").
+      { iApply ("Hk" with "Hpromise_inv"). iExists m. by iFrame. }
       { by auto. }
   }
-  (* ************************************************************************ *)
+  (* ************************************************************** *)
 
   iApply (Ectxi_ewp_bind (AppLCtx _)). done.
   iApply ewp_pure_step. apply pure_prim_step_rec.
@@ -446,19 +492,19 @@ Proof.
   iApply ewp_pure_step. apply pure_prim_step_beta. simpl.
   iApply (ewp_bind (ConsCtx (AppLCtx _) (ConsCtx (AppRCtx _) EmptyCtx))). done.
   iApply ewp_mono'; [
-  iApply (promise_alloc _ (W_inv q (Ready q)) Φ) |]. simpl.
+  iApply (promise_alloc q (ready q) Φ) |]. simpl.
   iModIntro. iIntros (v) "H".
-  iDestruct "H" as (p γ) "(-> & Hrunning & Hpromise_inv)".
-  iMod (promise_upd with "[$]") as "[Hhandler Hp]".
-  iAssert (∃ n, is_queue q (Ready q) n)%I with "[Hq]" as "Hq".
+  iDestruct "H" as (p γ) "(-> & Hrunning & Hpoints_to)".
+  iMod (promise_upd with "[$]") as "[Hpromise_inv Hp]".
+  iAssert (∃ (n : nat), is_queue q (ready q) n)%I with "[Hq]" as "Hq".
   { by iExists 0%nat. }
   iModIntro.
 
-  (* ************************************************************************ *)
+  (* ************************************************************** *)
   (** Verification of [fulfill]. *)
 
   (* Step 1 - Löb induction. *)
-  iLöb as "IH" forall (γ p Φ main). iDestruct "Hp" as "#Hp".
+  iLöb as "IH" forall (main q p γ Φ).
 
   iApply (Ectxi_ewp_bind (AppLCtx _)). done.
   iApply ewp_pure_step. apply pure_prim_step_beta. simpl.
@@ -471,68 +517,63 @@ Proof.
   iApply (ewp_bind (ConsCtx (AppLCtx _) (ConsCtx (AppRCtx _) EmptyCtx))). done.
   iApply ewp_pure_step. apply pure_prim_step_rec.
   iApply ewp_value. simpl.
-  iDestruct "Hq" as (n) "Hq".
 
   (* Step 2 - Reasoning rule for deep handlers. *)
   iApply (ewp_deep_try_with with "Hmain").
 
-  (* Step 3 - Proof of [is_deep_hanlder] judgement. *)
-  iAssert (▷ is_queue q (Ready q) n)%I with "Hq" as "Hq".
-  iRevert "Hp". iLöb as "IH_handler" forall (n Φ γ p). iIntros "#Hp".
+  (* Step 3 - Proof of [is_deep_hanlder] judgment. *)
+  iAssert (▷ ∃ (n : nat), is_queue q (ready q) n)%I with "Hq" as "Hq".
+  iLöb as "IH_handler" forall (q p γ Φ).
   rewrite deep_handler_unfold.
   iSplit.
 
   (* Return branch. *)
   - iIntros (v) "#Hv".
-    iDestruct (promise_agree with "[$]") as (S) "(HS & Hinv & H)".
-    iDestruct "H" as (Ψ) "(% & Hpromise_inv & H)".
-    rename H into Hlookup.
-    iDestruct (promise_unfold_equiv with "H") as "#Heq". iNext.
-    iApply ewp_pure_step. apply pure_prim_step_beta. simpl.
-    iDestruct "Hpromise_inv" as (b) "[Hrunning' Hp_inv]".
-    iPoseProof (running_agree with "[$]") as "%". rewrite H. clear H.
-    iDestruct "Hp_inv" as (l ks) "(Href & Hl & HW_inv)".
+    iDestruct (promise_agree q (ready q) with "[$]") as (S) "(HS & Hinv & H)".
+    iDestruct "H" as (Ψ) "(% & Hpoints_to & Heq')".
+    rename H into lookup_S.
+    iDestruct "Hpoints_to" as (b) "[Hrunning' Hp]".
+    iDestruct (running_agree with "[$]") as "%". rewrite H; clear H.
+    iDestruct "Hp" as (l ks) "(Hp & Hl & Hks)".
+    iPoseProof (promise_unfold_equiv with "Heq'") as "#Heq". iClear "Heq'".
+    iNext. iApply ewp_pure_step. apply pure_prim_step_beta. simpl.
     iApply (Ectxi_ewp_bind (CaseCtx _ _)). done.
-    iApply (ewp_mono' with "[Href]").
-    iApply (ewp_load with "Href").
-    simpl. iIntros (w) "[-> Href]".
+    iApply (ewp_mono' with "[Hp]"). { by iApply (ewp_load with "Hp"). }
+    iIntros (w) "[-> Hp]".
     iApply ewp_pure_step. apply pure_prim_step_case_InjR.
     iApply (Ectxi_ewp_bind (AppLCtx _)). done.
     iApply ewp_pure_step. apply pure_prim_step_rec.
     iApply ewp_value. simpl.
     iApply ewp_pure_step. apply pure_prim_step_beta. simpl.
     iApply (Ectxi_ewp_bind (AppRCtx _)). done.
-    iApply (ewp_mono' with "[HW_inv Hl Hq]").
-    { iApply (ewp_bind (ConsCtx (AppLCtx _) (ConsCtx (AppRCtx _) EmptyCtx))). done.
+    iApply (ewp_mono' with "[Hks Hl Hq]").
+    { iApply (ewp_bind (ConsCtx (AppLCtx _)
+                       (ConsCtx (AppRCtx _) EmptyCtx))). done.
+      iApply ewp_pure_step. apply pure_prim_step_rec. simpl.
+      iApply ewp_value.
+      iApply (list_iter_spec' _
+             (λ fs, (∃ (n : nat), is_queue q (ready q) n) ∗
+                    ([∗ list] f ∈ fs, ∀ (v : val), □ Ψ v -∗
+                       ▷ promise_inv q (ready q) -∗
+                         ▷ (∃ (n : nat), is_queue q (ready q) n) -∗
+                           EWP (f : val) v <|⊥|> {{ _, True }}))%I _ _ ks with "[] Hl");
+      [|by iFrame].
+      iModIntro. iIntros (gs f fs <-) "[Hq Hfs]".
+      rewrite big_opL_cons. iDestruct "Hfs" as "[Hf Hfs]".
+      iAssert (ready q (λ: <>, f v)%V)%I with "[Hf]" as "Hready".
+      { rewrite ready_unfold. iIntros "Hpromise_inv Hq".
+        iApply ewp_pure_step. apply pure_prim_step_beta. simpl.
+        iApply ("Hf" with "[] Hpromise_inv Hq"). by iRewrite ("Heq" $! v).
+      }
+      iDestruct "Hq" as (n) "Hq".
+      iApply ewp_pure_step. apply pure_prim_step_beta. simpl.
+      iApply (Ectxi_ewp_bind (AppRCtx _)). done.
       iApply ewp_pure_step. apply pure_prim_step_rec.
       iApply ewp_value. simpl.
-      iApply (list_iter_spec _
-             (λ ys, (∃ n : natO, is_queue q (Ready q) n) ∗
-                    ([∗ list] f ∈ (drop (length ys) ks),
-                      ▷ W_inv q (Ready q) Ψ f))%I _ _ ks with "[] [Hl]").
-      - iModIntro. iIntros (ks' k vs <-) "[Hq HI]".
-        rewrite -app_assoc -cons_middle drop_app big_opL_cons.
-        iDestruct "HI" as "[Hk HI]". iDestruct "Hq" as (m) "Hq".
-        iApply ewp_pure_step'. apply pure_prim_step_beta. simpl.
-        iNext. iApply (ewp_mono' with "[Hq Hk]").
-        iApply (Ectxi_ewp_bind (AppRCtx _)). done.
-        iApply ewp_pure_step. apply pure_prim_step_rec.
-        iApply ewp_value. simpl.
-        iApply (queue_push_spec with "Hq [Hk]").
-        { iNext. rewrite !Ready_unfold /Ready_pre !W_inv_unfold /W_inv_pre.
-          iIntros "Hhandler Hq". iDestruct "Hq" as (n') "Hq".
-          iApply ewp_pure_step'. apply pure_prim_step_beta. simpl. iNext.
-          iApply ("Hk" with "Hhandler [Hq]").
-          - by iExists n'. - by iRewrite ("Heq" $! v).
-        }
-        simpl. iIntros (_) "Hq". iSplitL "Hq"; [ by iExists (Datatypes.S m) |].
-        rewrite (cons_middle k ks' vs) app_assoc  drop_app.
-        iModIntro. iApply (big_sepL_mono with "HI"). by auto.
-      - done.
-      - iNext. rewrite drop_0. iSplitL "Hq".
-        by eauto. iApply (big_sepL_mono with "HW_inv"). by auto.
+      iApply (ewp_mono' with "[Hq Hready]"). { by iApply (queue_push_spec with "Hq Hready"). }
+      iIntros (_) "Hq". iModIntro. by eauto with iFrame.
     }
-    simpl. iModIntro. iIntros (w) "(_ & Hq & _)".
+    iModIntro. iIntros (w) "(_ & Hq & _)".
     iApply (Ectxi_ewp_bind (AppLCtx _)). done.
     iApply ewp_pure_step. apply pure_prim_step_rec.
     iApply ewp_value. simpl.
@@ -541,35 +582,27 @@ Proof.
     iApply (Ectxi_ewp_bind (StoreRCtx _)). done.
     iApply ewp_pure_step. apply pure_prim_step_InjL.
     iApply ewp_value. simpl.
-    iApply (ewp_mono' with "[Href]").
-    iApply (ewp_store with "Href"). simpl. iModIntro.
-    iIntros (w') "Href".
+    iApply (ewp_mono' with "[Hp]"). { by iApply (ewp_store with "Hp"). }
+    iModIntro. iIntros (u) "Hp".
+    iMod (running_upd _ _ _ false with "Hrunning' Hrunning") as "[Hrunning' Hrunning]".
+    iAssert (points_to q (ready q) p γ Ψ) with "[Hp Hrunning']" as "Hpoints_to".
+    { iExists false. iFrame. iExists v. iFrame. by iRewrite ("Heq" $! v). }
+    iAssert (promise_inv q (ready q)) with "[HS Hinv Hpoints_to]" as "Hpromise_inv".
+    { rewrite promise_inv_unfold. iExists S. iFrame.
+      rewrite (big_sepM_delete _ S (p, γ) _ lookup_S). by iFrame. }
     iApply (Ectxi_ewp_bind (AppLCtx _)). done.
     iApply ewp_pure_step. apply pure_prim_step_rec.
     iApply ewp_value. simpl.
     iApply ewp_pure_step. apply pure_prim_step_beta. simpl.
-    iMod (running_upd _ _ _ false
-      with "Hrunning' Hrunning") as "[Hrunning' Hrunning]".
-    iAssert (promise_inv γ p (W_inv q (Ready q)) Ψ)%I
-      with "[Href Hrunning']" as "Hpromise_inv".
-    { iExists false. iFrame. iExists v.
-      iRewrite ("Heq" $! v). by iFrame. }
-    iAssert (handler_inv (W_inv q (Ready q)))%I
-      with "[HS Hinv Hpromise_inv]" as "Hhandler_inv".
-    { iExists S. iFrame.
-      rewrite (big_sepM_delete _ S (p, γ) _ Hlookup).
-      by iFrame. }
-    iModIntro. iClear "H Hp Hv Heq". iDestruct "Hq" as (n') "Hq".
-    iApply (ewp_mono' with "[Hhandler_inv Hq]").
-    iApply ("run_next_spec" $! n' with "[$] [$]"). by auto.
+    by iApply ("next_spec" with "Hpromise_inv Hq").
 
   (* Effect branch. *)
   - iIntros (v k) "Hprot_agr".
-    iDestruct (Ψ_concurrency_agreement with "Hprot_agr") as "[Hasync|Hawait]".
+    iDestruct (Ψ_conc_agreement with "Hprot_agr") as "[Hasync|Hawait]".
 
     (* Async. *)
-    + rewrite Ψ_async_agreement. iNext. iApply fupd_ewp.
-      iMod "Hasync" as (e Φ') "(-> & He & Hk)".
+    + iClear "next_spec". rewrite Ψ_async_agreement. 
+      iDestruct "Hasync" as (e Φ') "(-> & He & Hk)".
       iApply (Ectxi_ewp_bind (AppLCtx _)). done.
       iApply ewp_pure_step. apply pure_prim_step_beta. simpl.
       iApply ewp_pure_step. apply pure_prim_step_rec.
@@ -581,65 +614,59 @@ Proof.
       iApply ewp_value. simpl.
       iApply ewp_pure_step. apply pure_prim_step_beta. simpl.
       iApply (Ectxi_ewp_bind (AppRCtx _)). done.
-      iApply ewp_mono'.
-      iApply (promise_alloc _ (W_inv q (Ready q)) Φ').
-      iModIntro. simpl. iIntros (_p') "Hp'". 
-      iDestruct "Hp'" as (p' γ') "(-> & Hrunning' & Hpromise_inv)".
-      iMod (promise_upd with "[$]") as "[Hhandler_inv #Hp']".
-      iMod ("Hk" $! p' with "[Hp']") as "Hk". { by iExists γ'. }
-      iModIntro.
+      iApply ewp_mono'. { by iApply (promise_alloc q (ready q) Φ'). }
+      iNext. iIntros (_p') "Hp'". simpl.
+      iDestruct "Hp'" as (p' γ') "(-> & Hrunning' & Hpoints_to)".
+      iMod (promise_upd with "[$]") as "[Hpromise_inv #Hp']". iModIntro.
+      iSpecialize ("Hk" $! p' with "[Hp']"). { by iExists γ'. }
       iApply (Ectxi_ewp_bind (AppLCtx _)). done.
       iApply ewp_pure_step'. apply pure_prim_step_rec.
       iNext. iApply ewp_value. simpl.
       iApply ewp_pure_step. apply pure_prim_step_beta. simpl.
       iApply (Ectxi_ewp_bind (AppRCtx _)). done.
-      iApply (ewp_mono' with "[Hq Hk Hrunning]").
-      { iApply (Ectxi_ewp_bind (AppRCtx _)). done.
-        iApply ewp_pure_step. apply pure_prim_step_rec.
-        iApply ewp_value. simpl.
-        iApply (queue_push_spec with "Hq"). iNext.
-        rewrite Ready_unfold /Ready_pre.
-        iIntros "Hhandler_inv Hq".
-        iDestruct "Hq" as (n') "Hq".
-        iSpecialize ("IH_handler" with "Hrunning Hhandler_inv Hq Hp").
-        iApply ewp_pure_step'. apply pure_prim_step_beta.
-        iNext. simpl. by iApply "Hk".
-      }
-      simpl. iIntros (v) "Hq". iModIntro.
-      iApply (Ectxi_ewp_bind (AppLCtx _)). done.
-      iApply ewp_pure_step'. apply pure_prim_step_rec. iNext.
+      iApply (Ectxi_ewp_bind (AppRCtx _)). done.
+      iApply ewp_pure_step. apply pure_prim_step_rec.
       iApply ewp_value. simpl.
+      iAssert (ready q (λ: <>, k #p')%V)%I with "[Hk Hrunning Hp]" as "Hready".
+      { rewrite ready_unfold. iIntros "Hpromise_inv Hq".
+        iApply ewp_pure_step'. apply pure_prim_step_beta.
+        iNext. iApply "Hk".
+        by iApply ("IH_handler" with "Hrunning Hpromise_inv Hp Hq").
+      }
+      iDestruct "Hq" as (n) "Hq".
+      iApply (ewp_mono' with "[Hq Hready]").
+      { by iApply (queue_push_spec with "Hq Hready"). }
+      iIntros (v) "Hq". iModIntro.
+      iApply (Ectxi_ewp_bind (AppLCtx _)). done.
+      iApply ewp_pure_step. apply pure_prim_step_rec.
+      iApply ewp_value.
       iApply ewp_pure_step. apply pure_prim_step_beta. simpl.
-      iApply ("IH" with "He Hrunning' Hhandler_inv Hp'").
-      by iExists (Datatypes.S n).
+      by iApply ("IH" with "He Hrunning' Hpromise_inv Hp'"); eauto.
 
     (* Await. *)
-    + iClear "IH".
-      rewrite Ψ_await_agreement. iNext. iApply fupd_ewp.
-      iMod "Hawait" as (p' Φ') "(-> & #Hp' & Hk)".
-      iDestruct "Hp'" as (γ') "#Hp'".
-      iDestruct (promise_agree with "[Hhandler]") as (S) "(HS & Hinv & H)".
-      { iFrame. by iApply "Hp'". }
-      iDestruct "H" as (Ψ) "(% & Hpromise_inv & H)".
-      rename H into Hlookup.
-      iDestruct (promise_unfold_equiv with "H") as "#Heq'". iClear "H".
-      iDestruct "Hpromise_inv" as (b) "[Hrunning' Hpromise_inv]".
+    + iClear "IH". rewrite Ψ_await_agreement.
+      iDestruct "Hawait" as (p' Φ') "(-> & #His_promise & Hk)".
+      iDestruct "His_promise" as (γ') "#His_promise".
+      iDestruct (promise_agree with "[Hpromise_inv]") as (S) "(HS & Hinv & H)".
+      { by eauto with iFrame. }
+      iDestruct "H" as (Ψ) "(% & Hpoints_to & Heq')". rename H into lookup_S.
+      iDestruct (promise_unfold_equiv with "Heq'") as "#Heq". iClear "Heq'".
+      iDestruct "Hpoints_to" as (b) "[Hrunning' Hp']".
       iApply (Ectxi_ewp_bind (AppLCtx _)). done.
       iApply ewp_pure_step. apply pure_prim_step_beta. simpl.
       iApply ewp_pure_step. apply pure_prim_step_rec.
       iApply ewp_value. simpl.
       iApply ewp_pure_step. apply pure_prim_step_beta. simpl.
-      iApply ewp_pure_step'. apply pure_prim_step_case_InjR.
-      iModIntro. iNext. case b.
-      { iDestruct "Hpromise_inv" as (l ks) "(Href & Hl & HW_inv)".
-        iApply (Ectxi_ewp_bind (AppLCtx _)). done.
-        iApply ewp_pure_step'. apply pure_prim_step_rec. simpl.
-        iIntros "!>". iApply ewp_value. simpl.
-        iApply ewp_pure_step. apply pure_prim_step_beta. simpl.
+      iApply ewp_pure_step. apply pure_prim_step_case_InjR.
+      iApply (Ectxi_ewp_bind (AppLCtx _)). done.
+      iApply ewp_pure_step. apply pure_prim_step_rec. simpl.
+      iApply ewp_value.
+      iApply ewp_pure_step. apply pure_prim_step_beta. simpl.
+      iNext. case b.
+      { iDestruct "Hp'" as (l ks) "(Hp' & Hl & Hks)".
         iApply (Ectxi_ewp_bind (CaseCtx _ _)). done.
-        iApply (ewp_mono' with "[Href]").
-        iApply (ewp_load with "Href"). simpl.
-        iIntros (w) "[-> Href]".
+        iApply (ewp_mono' with "[Hp']"). { by iApply (ewp_load with "Hp'"). }
+        iIntros (w) "[-> Hp']". iModIntro. simpl.
         iApply ewp_pure_step. apply pure_prim_step_case_InjR.
         iApply (Ectxi_ewp_bind (AppLCtx _)). done.
         iApply ewp_pure_step. apply pure_prim_step_rec. simpl.
@@ -648,79 +675,49 @@ Proof.
         iApply (Ectxi_ewp_bind (AppRCtx _)). done.
         iApply (ewp_bind (ConsCtx (StoreRCtx _)
                          (ConsCtx  InjRCtx EmptyCtx))). done.
-        iApply (ewp_bind (ConsCtx (AppLCtx _)
-                         (ConsCtx (AppRCtx _) EmptyCtx))). done.
-        iApply ewp_pure_step. apply pure_prim_step_rec.
-        iApply ewp_value. simpl.
-        iApply (ewp_mono' with "[Hl]").
-        iApply (list_cons_spec with "Hl"). simpl.
-        iModIntro. iIntros (l') "Hl'".
+        iApply (ewp_mono' with "[Hl]"). { by iApply (list_cons_spec with "Hl"). }
+        iIntros (l') "Hl'". iModIntro. simpl.
         iApply (Ectxi_ewp_bind (StoreRCtx _)). done.
-        iApply ewp_pure_step'. apply pure_prim_step_InjR.
-        iModIntro. iNext.
+        iApply ewp_pure_step. apply pure_prim_step_InjR.
         iApply ewp_value. simpl.
-        iApply (ewp_mono' with "[Href]").
-        iApply (ewp_store with "Href"). simpl.
-        iIntros (w) "Href".
-        iAssert (W_inv q (Ready q) Ψ (λ: "x", k "x")%V)%I
-          with "[Hk Hrunning]" as "Hk".
-        { rewrite W_inv_unfold /W_inv_pre. iIntros (v) "Hhandler_inv Hq #Hv".
-          iSpecialize("Hk" $! v with "[]").
-          { iModIntro. by iRewrite -("Heq'" $! v). }
-          iApply fupd_ewp. iMod "Hk".
-          iApply ewp_pure_step'. apply pure_prim_step_beta. simpl.
-          iModIntro. iNext. iApply "Hk".
-          iDestruct "Hq" as (n') "Hq".
-          iSpecialize ("IH_handler" with "Hrunning Hhandler_inv Hq Hp").
-          by iApply "IH_handler".
-        }
-        iAssert (promise_inv γ' p' (W_inv q (Ready q)) Ψ)%I
-          with "[Href Hl' Hrunning' HW_inv Hk]" as "Hpromise_inv".
-        { iExists true. iFrame. iExists l', ((λ: "x", k "x")%V :: ks).
-          iFrame. iApply (big_sepL_mono with "HW_inv"). by auto. }
-        iAssert (handler_inv (W_inv q (Ready q)))%I
-          with "[HS Hinv Hpromise_inv]" as "Hhandler_inv".
-        { iExists S. iFrame.
-          rewrite (big_sepM_delete _ S (p', γ') _ Hlookup).
-          by iFrame. }
-        iModIntro.
+        iApply (ewp_mono' with "[Hp']"). { by iApply (ewp_store with "Hp'"). }
+        iIntros (w) "Hp'".
         iApply (Ectxi_ewp_bind (AppLCtx _)). done.
         iApply ewp_pure_step. apply pure_prim_step_rec. simpl.
-        iApply ewp_value. simpl.
+        iApply ewp_value.
         iApply ewp_pure_step. apply pure_prim_step_beta. simpl.
-        by iApply ("run_next_spec" with "Hhandler_inv Hq").
+        iAssert (points_to q (ready q) p' γ' Ψ)
+        with "[Hrunning Hp Hrunning' Hks Hl' Hp' Hk]" as "Hpoints_to".
+        { iExists true. iFrame. iExists l', (_ :: ks). iFrame.
+          iIntros (v) "#HΨ Hpromise_inv Hq". iRewrite ("Heq" $! v) in "HΨ".
+          iSpecialize ("Hk" with "HΨ").
+          iApply "Hk". iNext.
+          by iApply ("IH_handler" with "Hrunning Hpromise_inv Hp Hq").
+        }
+        iAssert (promise_inv q (ready q))%I with "[HS Hinv Hpoints_to]" as "Hpromise_inv".
+        { rewrite promise_inv_unfold. iExists S. iFrame.
+          rewrite (big_sepM_delete _ S (p', γ') _ lookup_S). by iFrame.
+        }
+        by iApply ("next_spec" with "Hpromise_inv Hq").
       }
-      { iDestruct "Hpromise_inv" as (v) "[Href #Hv]".
-        iSpecialize("Hk" $! v with "[]").
-        { iModIntro. by iRewrite -("Heq'" $! v). }
-        iApply fupd_ewp. iMod "Hk". iModIntro.
-        iApply (Ectxi_ewp_bind (AppLCtx _)). done.
-        iApply ewp_pure_step'. apply pure_prim_step_rec. simpl.
-        iIntros "!>". iSpecialize ("Hk" $! ⊥%ieff (λ _, True%I)).
-        iApply ewp_value. simpl.
-        iApply ewp_pure_step. apply pure_prim_step_beta. simpl.
+      { iDestruct "Hp'" as (v) "[Hp' #Hv]".
+        iRewrite ("Heq" $! v) in "Hv". iSpecialize("Hk" $! v with "Hv").
         iApply (Ectxi_ewp_bind (CaseCtx _ _)). done.
-        iApply (ewp_mono' with "[Href]").
-        iApply (ewp_load with "Href"). simpl.
-        iIntros (w) "[-> Href]".
-        iAssert (promise_inv γ' p' (W_inv q (Ready q)) Ψ)%I
-          with "[Href Hrunning']" as "Hpromise_inv".
-        { iExists false. iFrame. iExists v. by iFrame. }
-        iAssert (handler_inv (W_inv q (Ready q)))%I
-          with "[HS Hinv Hpromise_inv]" as "Hhandler_inv".
-        { iExists S. iFrame.
-          rewrite (big_sepM_delete _ S (p', γ') _ Hlookup).
-          by iFrame. }
-        iSpecialize ("IH_handler" with "Hrunning Hhandler_inv Hq Hp").
-        iSpecialize("Hk" with "IH_handler").
+        iApply (ewp_mono' with "[Hp']"). { by iApply (ewp_load with "Hp'"). }
+        iIntros (w) "[-> Hp']". simpl.
         iModIntro. iApply ewp_pure_step. apply pure_prim_step_case_InjL.
         iApply (Ectxi_ewp_bind (AppLCtx _)). done.
         iApply ewp_pure_step. apply pure_prim_step_rec.
         iApply ewp_value. simpl.
-        iApply ewp_pure_step. apply pure_prim_step_beta.
-        by iApply "Hk".
+        iApply ewp_pure_step'. apply pure_prim_step_beta. simpl.
+        iNext. iApply "Hk".
+        iApply ("IH_handler" with "Hrunning [HS Hinv Hrunning' Hp'] Hp Hq").
+        iAssert (points_to q (ready q) p' γ' Ψ)%I with "[Hrunning' Hp']" as "Hpoints_to".
+        { iExists false. iFrame. iExists v. iRewrite ("Heq" $! v). by iFrame. }
+        rewrite promise_inv_unfold. iExists S. iFrame.
+        rewrite (big_sepM_delete _ S (p', γ') _ lookup_S). by iFrame.
       }
-  (* ************************************************************************ *)
+  (* ************************************************************** *)
 Qed.
 
 End scheduler.
@@ -736,22 +733,22 @@ Context `{!inG Σ (authR (gmapUR
                           (loc * gname)
                           (agreeR (laterO (val -d> (iPrePropO Σ))))))}.
 
-Lemma handler_inv_alloc : ⊢ |==> ∃ γ, ∀ W_inv, handler_inv γ W_inv.
+Lemma promise_inv_alloc : ⊢ |==> ∃ γ, ∀ q ready, promise_inv γ q ready.
 Proof.
-  iIntros.
-  iMod (own_alloc (● (∅ : gmap (loc * gname) _))) as (γI) "HI";
+  iIntros. iMod (own_alloc (● (∅ : gmap (loc * gname) _))) as (γI) "HI";
     first by rewrite auth_auth_valid.
-  iModIntro. iExists γI. iIntros (W_inv).
+  iModIntro. iExists γI. iIntros (q ready).
+  rewrite promise_inv_unfold.
   iExists ∅. rewrite fmap_empty. by iFrame.
 Qed.
 
 Lemma run_spec (main : val) : ⊢ |==> ∃ γ,
-  EWP main #() @ ∅ <| Ψ_concurrency γ |> {{ _, True }} -∗
-    EWP run main @ ∅ {{ _, True }}.
+  EWP main #() <| Ψ_conc γ |> {{ _, True }} -∗
+    EWP run main {{ _, True }}.
 Proof.
-  iMod handler_inv_alloc as (γ) "Hhandler_inv".
+  iMod promise_inv_alloc as (γ) "Hpromise_inv".
   iModIntro. iExists γ. iIntros "Hmain".
-  iApply (run_spec' _ _ (λ _, True%I) with "Hhandler_inv").
+  iApply (run_spec' _ _ (λ _, True%I) with "Hpromise_inv").
   iApply (ewp_mono with "Hmain"). by auto.
 Qed.
 
